\documentclass[a4paper]{article}

\usepackage{fullpage} % Package to use full page
\usepackage{parskip} % Package to tweak paragraph skipping
\usepackage{tikz} % Package for drawing
\usepackage{amsmath}
\usepackage{hyperref}
\usepackage{amssymb}

\usepackage{enumitem}

\title{Chapter 9 Generating Functions}
\author{Ling Tan}
\date{2018/09}

\begin{document}

\maketitle

\section*{4.2 Recursive Definitions}
\color{red}e.g.: \color{black} $\binom{n+1}{r}=\binom{n}{r}+\binom{n}{r-1}, n\geq r\geq 0$
\begin{itemize}
    \item Combinatorial proof \\
    LHS: choose $r$ from $n+1$\\
    RHS: take $1$ from $n+1$, this $1$ either in $r$ or not in $r$\\
\end{itemize}

\color{red}e.g.: \color{black} $\binom{m+n}{r}=\sum_{k=0}^{r}{\binom{m}{r-k}\binom{n}{k}}$
\begin{align*}
\text{Let }&|A|=m,|B|=n,A\cap B=\emptyset\\
\Rightarrow& |{A \cup B}|=m+n\\
\text{Select $r$ elements from }& {A \cup B}
\end{align*}

\color{red}e.g.: \color{black}$\binom{n+1}{r+1}=\sum_{j=r}^{n}{\binom{j}{r}}$
\begin{align*}
\binom{n+1}{r+1}&=\binom{n}{r+1}+\binom{n}{r}\\
&=\binom{n-1}{r+1}+\binom{n-1}{r}+\binom{n}{r}\\
&=\binom{n-2}{r+1}+\binom{n-2}{r}+\binom{n-1}{r}+\binom{n}{r}\\
&=\binom{n-3}{r+1}+\binom{n-3}{r}+\binom{n-2}{r}+\binom{n-1}{r}+\binom{n}{r}\\
&=\binom{r+1}{r+1}+\binom{r+1}{r}+\binom{r+2}{r}+\cdots+\binom{n}{r}\\
&=\binom{r}{r}+\binom{r+1}{r}+\binom{r+2}{r}+\cdots+\binom{n}{r}\\
&=\sum_{j=r}^{n}{\binom{j}{r}}
\end{align*}

\end{document}